\newpage

\section{Gamma Function}

$\Gamma(z) \myeq \int_{0}^{\infty} t^{z-1} e^{-t}\ dt .$ 

\noindent $\Gamma(z)$ can be analytically continued to $\mathbb{C}$ except for
poles at $S=\{0, -1, -2, -3, \cdots \}$ with residue $\frac{(-1)^n}{n!}$ at
$s=-n$.

Representations of $\Gamma(z)$:

$$\Gamma(z) = \lim_{n->\infty} \frac{n^{z}n!}{z(z+1)(z+2) \cdots (z+n)}$$

$$\frac{1}{\Gamma(z)} = z e^{\gamma z} \prod_{n=1}^{\infty}
(1+\frac{z}{n})e^{-\frac{z}{n}}$$
for all z, and where $\gamma$ is Euler's gamma constant. ( Product Formula ).

Functional equations of $\Gamma(z)$:

$$\Gamma(z+1) = z \Gamma(z)$$

$$\Gamma(z)\Gamma(1-z) = \frac{\pi}{\sin{(\pi z)}}$$


[ TBD: ]

Wielandt's Theorem can derive:

- the GAUSS product from the EULER integral,

- the multiplication formulae of GAUSS,

- the representation of the Beta function by Gamma functions,

- STIRLING s formula.


\section{Zeta Function}

$$\zeta(s) = \sum_{n=1}^\infty\frac{1}{n^s} = 1+\frac{1}{2^s}+\frac{1}{3^s}+\frac{1}{4^s}+\frac{1}{5^s}+ \ldots$$

\subsection{Euler's Product Formula}

$$\zeta(s) = \sum_{n=1}^\infty\frac{1}{n^s} = \prod_{p \text{ prime}} \frac{1}{1-p^{-s}}$$

$$\prod_{p \text{ prime}} \frac{1}{1-p^{-s}} = \frac{1}{1-2^{-s}}\cdot\frac{1}{1-3^{-s}}\cdot\frac{1}{1-5^{-s}}\cdot\frac{1}{1-7^{-s}} \cdots \frac{1}{1-p^{-s}} \cdots$$

$$ \frac{1}{1-p^{-s}} = 1 + \frac{1}{p^s} + \frac{1}{p^{2s}} + \frac{1}{p^{3s}} + \ldots + \frac{1}{p^{ks}} + \ldots $$ 


[ TBD: ]

Show that LHS = RHS.

Number subsections.


\section{Inverse Zeta Function / Moebius Mu Function}
